rocq/Ender/Syntax.v
@@ -55,7 +55,8 @@ Inductive Reason :=
 | EquilatEquiang : nat -> Reason
 | EquiangEquilat : nat -> Reason
 | ConSupplements : nat -> nat -> nat -> Reason
-| ConSupplementsSame : nat -> nat -> Reason.
+| ConSupplementsSame : nat -> nat -> Reason
+| DefPerp : nat -> Reason.
 
 Record Premise := premise { premise_label : string; premise_statement : Statement }.
 Record Step := step { step_reason : Reason; step_conclusion : Statement }.
